src/Progress.v
@@ -1,0 +1,99 @@
+Require Import HJ.Vars.
+
+Module Request.
+
+Record request {O:Type} := mk_request {
+  reqs : Map_TID.t O;
+  Check: tid -> O -> Prop;
+  In : tid -> Prop
+}.
+
+Implicit Arguments reqs.
+Implicit Arguments Check.
+Implicit Arguments In.
+Implicit Arguments mk_request.
+End Request.
+
+Module RequestSpec.
+Record request_spec
+  {O:Type} 
+  (reqs : Vars.Map_TID.t O)
+  (Check: tid -> O -> Prop)
+  (In : tid -> Prop)
+:= {
+  (** We only consider operations from task in the state. *)
+  reqs_in:
+    forall t,
+    In t <-> Map_TID.In t reqs;
+  (** All requests are valid. *)
+  reqs_check:
+    forall t o,
+    Map_TID.MapsTo t o reqs -> Check t o
+}.
+Implicit Arguments reqs_in.
+Implicit Arguments reqs_check.
+End RequestSpec.
+
+Section ProgressProp.
+Variable O:Type.
+Variable reqs : Map_TID.t O.
+Variable Check: tid -> O -> Prop.
+Variable In : tid -> Prop.
+Variable reqs_spec : RequestSpec.request_spec reqs Check In.
+Variable S:Type.
+(** The state. *)
+Variable state : S.
+(** The given task issues an operation that yields a new state. *)
+Variable Reduce : tid -> O -> S -> Prop.
+(** Returns [true] when the given operation is blocking, [false] if unblocking. *)
+Variable blocking : O -> bool.
+
+Record progress_spec
+:= mk_progress_spec {
+  (** Any valid unblocked operation must be able to reduce. *)
+  progress_unblocked:
+    forall t o,
+    Check t o ->
+    blocking o = false ->
+    exists s', Reduce t o s';
+  (**
+    If all our requests are blocking requests, then there is at least
+    one that can be issued.
+  *)
+  progress_blocked:
+    (** The [state] must be nonempty. *)
+    ~ Map_TID.Empty reqs ->
+    (** All available requests are blocking. *)
+    (forall t o, Map_TID.MapsTo t o reqs -> blocking o = true) ->
+    (** There is a task that can reduce. *)
+    exists t o,
+    Map_TID.MapsTo t o reqs /\ exists s', Reduce t o s' 
+}.
+Implicit Arguments progress_unblocked.
+Implicit Arguments progress_blocked.
+
+Lemma main_progress:
+  forall (p:progress_spec),
+  ~ Map_TID.Empty reqs ->
+  (** There is a task that can reduce. *)
+  exists t o,
+  Map_TID.MapsTo t o reqs /\ exists s', Reduce t o s'.
+Proof.
+  intros.
+  destruct (Map_TID_Extra.pred_choice reqs (fun (_:tid) (o:O) => (negb (blocking o)))).
+  - auto with *. (* Proper *)
+  - destruct e as (t, (o, (Hmt, Hb))).
+    remember (blocking o) as b.
+    destruct b.
+    + inversion Hb.
+    + exists t.
+      exists o.
+      intuition.
+      apply (progress_unblocked); auto.
+      apply (RequestSpec.reqs_check reqs_spec); auto.
+  - apply (progress_blocked p); auto.
+    intros.
+    apply e in H0.
+    destruct (blocking o); auto.
+Qed.
+End ProgressProp.
